\documentclass[a4paper,11pt]{article}
\usepackage[cm]{fullpage}
\usepackage{amsmath}
\usepackage{amsfonts}

\newcommand{\of}[1]{\left( {#1} \right)}
\newcommand{\ofs}[1]{\left[ {#1} \right]}
\newcommand{\fracd}[2]{\frac{\dd{}{#1}}{\dd{}{#2}}}
\newcommand{\fracp}[2]{\frac{\partial{}{#1}}{\partial{}{#2}}}

\newcommand{\dd}{\text{d}}
\newcommand{\ee}{\text{e}}

\begin{document}
\section*{Logistic Regression Gradient Descent}
The notation of the video reads:
\[
\begin{split}
z & = w^T x + b,\\
\hat y &= a = \sigma\of{z}, \qquad \sigma\of{z} := \frac{1}{1 + \ee^{-z}}
\end{split}
\]
and the loss function
\[
\mathcal{L}\of{\hat{y}, y} = - \ofs{y \log\hat{y} + \of{1 - y} \log \of {1 - \hat{y}}}.
\]
Here, $x \in \mathbb{R}^{n_x}$ is a $n_x$-dimensional feature vector,
$w \in \mathbb{R}^{n_x}$ are $n_x$ weights, $b$ is the bias, $\hat{y}
\in [0, 1]$ is the prediction of the model based on $x$, and $y$ is
the ground truth label.

\subsection*{Derivative of the sigmoid function}
The derivative of $\sigma\of{z}$ with respect to its argument reads
\[
\begin{split}
\fracd{\sigma\of{z}}{z} &= \fracd{}{z}\of{\frac{1}{1 + \ee^{-z}}}
                        = \frac{\ee^{-z}}{\of{1 + \ee^{-z}}^2}
                        = \frac{\ee^{-z}}{1 + \ee^{-z}} \times \frac{1}{1 + \ee^{-z}}
                        = \frac{1 + \ee^{-z} - 1}{1 + \ee^{-z}} \times \frac{1}{1 + \ee^{-z}} =\\
                        &= \ofs{1 - \sigma\of{z}} \sigma\of{z}.
\end{split}
\]

\subsection*{Derivative of the loss function}
The derivative of $\mathcal{L}\of{\hat{y}, y}$ with resepect to the prediction $\hat{y}$ reads:
\[
\begin{split}
\fracp{}{\hat{y}} \mathcal{L}\of{\hat{y}, y} &=
- \fracp{}{\hat{y}} \ofs{y \log\hat{y} + \of{1 - y} \log\of{1 - \hat{y}}} =
- \of{\frac{y}{\hat{y}} - \frac{1 - y}{1 - \hat{y}}} =
- \frac{y\of{1-\hat{y}} - \hat{y}\of{1-y}}{\hat{y}\of{1 - \hat{y}}} = \\
&=
- \frac{y - y\hat{y} - \hat{y} + \hat{y}y}{\hat{y}\of{1 - \hat{y}}} =
  \frac{\hat{y} - y}{\hat{y}\of{1 - \hat{y}}} =
  \frac{\sigma\of{z} - y}{\sigma\of{z}\of{1 - \sigma\of{z}}}.
\end{split}
\]

\subsection*{Derivative $\partial\mathcal{L}_{\partial z}$}
For the derivative of the loss $\mathcal{L}$ with respect to $z$ we
consequently have
\[
\fracp{\mathcal{L}}{z} =
\fracp{\mathcal{L}}{\hat{y}} \fracd{\hat{y}}{z} =
\frac{\sigma\of{z} - y}{\sigma\of{z}\of{1 - \sigma\of{z}}} \times \of{1 - \sigma\of{z}}\sigma\of{z} = 
\sigma\of{z} - y.
\]
\end{document}
